\begin{problem}[习题2.4]
证明(以下四题任选两题)
\begin{enumerate}
\item $\displaystyle
\int_0^1 \mathrm{e}^{-xt}\ln(2+t)dt \sim \frac{\ln 2}{x}
$
\item $\displaystyle
\int_0^1 \mathrm{e}^{-xt}\ln(1+t)dt \sim \frac{1}{x^2}
$
\item $\displaystyle
\int_0^1 \mathrm{e}^{-xt}\sin tdt \sim \frac{1}{x^2}
$
\item $\displaystyle
\int_0^1\mathrm{e}^{-(x/t)+t+xt}dt \sim \frac{\mathrm{e}}{2x}
$
\end{enumerate}
\end{problem}

\begin{solution}
\begin{enumerate}
\item 由分步积分有
\begin{align*}
\int_{0}^{1}\mathrm{e}^{-xt}\ln(2+t)dt & =-\frac{1}{x}\bigg[\mathrm{e}^{-xt}\ln(2+t)\Big|_{0}^{1}-\int_{0}^{1}\frac{1}{\mathrm{e}^{xt}(2+t)}dt\bigg]\\
 & =-\frac{1}{x}\bigg[\mathrm{e}^{-x}\ln3-\ln2-\int_{0}^{1}\frac{1}{\mathrm{e}^{xt}(2+t)}dt\bigg]\\
 & =\frac{\ln2}{x}-\underbrace{\frac{\ln3}{x\mathrm{e}^{x}}}_{(a)}+\underbrace{\frac{1}{x}\int_{0}^{1}\frac{1}{\mathrm{e}^{xt}(2+t)}dt}_{(b)}
\end{align*}
其中(a)项$\ln3/(x\mathrm{e}^{x})=o(1/x)$. 其中(b)项
\[
\Bigg|\frac{1}{x}\int_{0}^{1}\frac{1}{\mathrm{e}^{xt}(2+t)}dt\Bigg|\le\Bigg|\frac{1}{2x}\int_{0}^{1}\mathrm{e}^{-xt}dt\Bigg|=\Bigg|\frac{1}{2x^{2}}\big(\mathrm{e}^{-x}-1\big)\Bigg|=o(1/x)
\]
因此
\[
\int_{0}^{1}\mathrm{e}^{-xt}\ln(2+t)dt=\frac{\ln2}{x}+o(1/x)\sim\frac{\ln2}{x}
\]

\item 由分步积分
\begin{align*}
\int_{0}^{1}\mathrm{e}^{-xt}\ln(1+t)dt & =-\frac{1}{x}\bigg[\mathrm{e}^{-xt}\ln(1+t)\Big|_{0}^{1}-\int_{0}^{1}\frac{1}{\mathrm{e}^{xt}(1+t)}dt\bigg]\\
 & =-\frac{1}{x}\bigg[\mathrm{e}^{-x}\ln2-0-\int_{0}^{1}\frac{1}{\mathrm{e}^{xt}(1+t)}dt\bigg]\\
 & =-\frac{\ln2}{x\mathrm{e}^{x}}+\frac{1}{x}\int_{0}^{1}\frac{1}{\mathrm{e}^{xt}(1+t)}dt\\
 & =-\frac{\ln2}{x\mathrm{e}^{x}}-\frac{1}{x^{2}}\bigg[\frac{1}{\mathrm{e}^{xt}(1+t)}\bigg|_{0}^{1}+\int_{0}^{1}\mathrm{e}^{-xt}\frac{1}{(1+t)^{2}}dt\bigg]\\
 & =-\frac{\ln2}{x\mathrm{e}^{x}}-\frac{1}{x^{2}}\bigg[\frac{1}{2\mathrm{e}^{x}}-1+\int_{0}^{1}\mathrm{e}^{-xt}\frac{1}{(1+t)^{2}}dt\bigg]\\
 & =\frac{1}{x^{2}}-\underbrace{\frac{\ln2}{x\mathrm{e}^{x}}}_{(a)}-\underbrace{\frac{1}{2x^{2}\mathrm{e}^{x}}}_{(b)}-\underbrace{\frac{1}{x^{2}}\int_{0}^{1}\mathrm{e}^{-xt}\frac{1}{(1+t)^{2}}dt}_{(c)}
\end{align*}
其中(a)和(b)项都是$o(1/x^{2})$. 其中(c)项
\[
\Bigg|\frac{1}{x^{2}}\int_{0}^{1}\mathrm{e}^{-xt}\frac{1}{(1+t)^{2}}dt\Bigg|\leq\frac{1}{4x^{2}}\int_{0}^{1}\mathrm{e}^{-xt}dt=o(1/x^{2})
\]
因此
\[
\int_{0}^{1}\mathrm{e}^{-xt}\ln(1+t)dt=\frac{1}{x^{2}}+o(1/x^{2})\sim\frac{1}{x^{2}}
\]

\item 由分步积分
\begin{align*}
\int_{0}^{1}\mathrm{e}^{-xt}\sin tdt & =-\frac{1}{x}\bigg[\mathrm{e}^{-xt}\sin t\big|_{0}^{1}-\int_{0}^{1}\mathrm{e}^{-xt}\cos tdt\bigg]\\
 & =-\frac{1}{x}\bigg\{\mathrm{e}^{-x}\sin1+\frac{1}{x}\Big[\mathrm{e}^{-xt}\cos t\Big|_{0}^{1}-\int_{0}^{1}\mathrm{e}^{-xt}\sin tdt\Big]\bigg\}\\
 & =-\frac{1}{x}\bigg\{\mathrm{e}^{-x}\sin1+\frac{1}{x}\Big[\mathrm{e}^{-x}\cos1-1-\int_{0}^{1}\mathrm{e}^{-xt}\sin tdt\Big]\bigg\}\\
 & =\frac{1}{x^{2}}\underbrace{-\frac{1}{x}\mathrm{e}^{-x}\sin1-\frac{1}{x^{2}}\mathrm{e}^{-x}\cos1}_{(a)}+\underbrace{\frac{1}{x^{2}}\int_{0}^{1}\mathrm{e}^{-xt}\sin tdt}_{(b)}
\end{align*}
其中(a)项为$o(1/x^{2})$. (b)项
\[
\bigg|\frac{1}{x^{2}}\int_{0}^{1}\mathrm{e}^{-xt}\sin tdt\bigg|\leq\bigg|\frac{1}{x^{2}}\int_{0}^{1}\mathrm{e}^{-xt}dt\bigg|=\bigg|\frac{1}{x^{3}}\Big(\mathrm{e}^{-x}-1\Big)\bigg|=o(1/x^{2})
\]
因此
\[
\int_{0}^{1}\mathrm{e}^{-xt}\sin tdt=\frac{1}{x^{2}}+o(1/x^{2})\sim\frac{1}{x^{2}}
\]
\end{enumerate}

\end{solution}
